Pyret.v
@@ -1,4 +1,5 @@
 Require Import Prelude.
+Require Import ListExt.
 Require Import Coq.ZArith.ZArith.
 Require Import Coq.Strings.String.
 
@@ -30,8 +31,7 @@ Ltac destruct_eq_dec a b :=
                  | [ H : ?x <> ?x |- _ ]
                    => exfalso; apply H; reflexivity end].
 
-
-Definition atom := Atom.t. (* free variables *)
+Definition atom := Atom.atom. (* free variables *)
 Definition loc := Atom.atom.
 Definition string := String.string.
 
@@ -50,12 +50,11 @@ Goal (if Atom.eq_dec __check__ __brand__ then 5 else 6) = 6.
 destruct_eq_dec __check__ __brand__.
   exfalso. apply check_brand_distinct; auto. Qed.
 
-
-Inductive brand : Type :=
+Inductive brand : Set :=
   | mkbrand : atom -> brand.
 
 Unset Elimination Schemes.
-Inductive exp : Type :=
+Inductive exp : Set :=
   | elam : list brand -> atom -> exp -> exp
   | eapp : exp -> exp -> exp
   | eid : atom -> exp
@@ -108,6 +107,8 @@ fix F (e : exp) : P e :=
   | egetfield a e => exp_rec_getfield a e (F e)
   end.
 
+Definition values l := map (@snd atom exp) l.
+
 Inductive value : exp -> Prop :=
   | vbool : forall l b, value (ebool l b)
   | vobj : forall l fs, Forall value (map snd fs) -> value (eobj l fs)
@@ -116,6 +117,66 @@ Inductive value : exp -> Prop :=
 
  Hint Constructors value.
 
+
+Inductive E : Set :=
+  | E_hole : E
+  | E_app1 : E -> exp -> E
+  | E_app2 : exp -> E -> E
+  | E_getfield : atom -> E -> E
+  | E_obj : forall (bs : list brand)
+                   (vs : list (atom * exp))
+                   (es : list (atom * exp)), 
+              (Forall value (values vs)) -> atom -> E -> E
+  | E_delta1 : atom -> E -> exp -> E
+  | E_delta2 : atom -> exp -> E -> E.
+
+
+Inductive ae : exp -> Prop :=
+  | redex_app  : forall e1 e2, value e1 -> value e2 -> ae (eapp e1 e2)
+  | redex_getfield : forall a e1, value e1 -> ae (egetfield a e1)
+  | redex_delta : forall a e1 e2, value e1 -> value e2
+                                  -> ae (edelta a e1 e2).
+
+
+Inductive decompose : exp -> E -> exp -> Prop :=
+  | ctxt_hole : forall e,
+      ae e ->
+      decompose e E_hole e
+  | ctxt_app1 : forall E e1 e2 e',
+      decompose e1 E e' ->
+      decompose (eapp e1 e2) (E_app1 E e2) e'
+  | ctxt_app2 : forall E v e e',
+      value v ->
+      decompose e E e' ->
+      decompose (eapp v e) (E_app2 v E) e'
+  | ctxt_getfield : forall a e E e',
+                      decompose e E e' ->
+                      decompose (egetfield a e) (E_getfield a E) e'
+  | ctxt_obj : forall bs vs es a e E e'
+                      (are_vals : Forall value (values vs)),
+      decompose e E e' ->
+      decompose (eobj bs (vs++(a,e)::es))
+                (E_obj bs vs es are_vals a E) e'
+  | ctxt_delta1 : forall a E e1 e2 e',
+                    decompose e1 E e' ->
+                    decompose (edelta a e1 e2) (E_delta1 a E e2) e'
+  | ctxt_delta2 : forall a v E e e',
+                    value v ->
+                    decompose e E e' ->
+                    decompose (edelta a v e) (E_delta2 a v E) e'.
+
+
+Fixpoint plug (e : exp) (cxt : E) := match cxt with
+  | E_hole => e
+  | E_app1 ctxt e2 => eapp (plug e ctxt) e2
+  | E_app2 v ctxt => eapp v (plug e ctxt)
+  | E_getfield a ctxt => egetfield a (plug e ctxt)
+  | E_obj bs vs es _ a ctxt => eobj bs (vs++(a,plug e ctxt)::es)
+  | E_delta1 a ctxt e => edelta a (plug e ctxt) e
+  | E_delta2 a v ctxt => edelta a v (plug e ctxt)
+  end.
+
+  
 SearchAbout sumbool.
 
 SearchAbout pair.
@@ -192,23 +253,30 @@ Fixpoint snoc {A:Type} (l:list A) (e:A) : list A :=
 
 SearchAbout nth.
 
+
 Inductive step : exp -> exp -> Prop :=
+  | sdecompose : forall e E e' e'',
+                   decompose e E e' ->
+                   step e' e''
+                   -> step e (plug e'' E)
   | sapp : forall x e b l,
              value e ->
              step (eapp (elam l x b) e)
                   (subst x e b)
   | sobj : forall bs vs a e e' es,
-             Forall value (map snd vs) ->
+             Forall value (values vs) ->
              Forall (fun x => ~ value x) (map snd es) ->
              ~ value e ->
              step e e' ->
              step (eobj bs (vs ++ (cons (a,e) es)))
                   (eobj bs (vs ++ (cons (a,e') es)))
   | sgetfield : forall bs vs a,
-                  Forall value (map snd vs) ->
+                  Forall value (values vs) ->
                   In a (map fst vs) ->
                   step (eobj bs vs)
-                       (GET THE FIELD)
+                       (* BAD: my default value is false *)
+                       (lookup_assoc vs a (ebool nil false)
+                                     Atom.eq_dec)
   | sdelta1 : forall a e1 e1' e2,
                step e1 e1' ->
                step (edelta a e1 e2) (edelta a e1' e2)
@@ -300,6 +368,21 @@ Example step_obj1 :
              ::nil))
     (eobj nil ((f1,ebool nil true)::(f2,ebool nil false)::nil)).
 Proof.
+  eapply multi_step.
+  Print sdecompose.
+  replace  ((f1,ebool nil true)
+             ::(f2, edelta __has_brand__
+                       (ebrand (mkbrand __some_brand__))
+                       (ebool nil true))
+             ::nil) with  ([(f1,ebool nil true)]
+             ++ ((f2, edelta __has_brand__
+                       (ebrand (mkbrand __some_brand__))
+                       (ebool nil true))
+             ::nil)) by auto.
+  eapply sdecompose.
+  eapply ctxt_obj.
+  eapply ctxt_hole.
+  
   rewrite fold_cons.
   rewrite <- app_split.
   eapply multi_step with
